statement of adequacy of coneris

theories/coneris/adequacy.v
@@ -8,9 +8,54 @@ From clutch.prelude Require Import stdpp_ext iris_ext.
 From clutch.con_prob_lang Require Import erasure notation.
 From clutch.common Require Export con_language sch_erasable.
 From clutch.base_logic Require Import error_credits.
-From clutch.coneris Require Import weakestpre.
+From clutch.coneris Require Import weakestpre primitive_laws.
 From clutch.prob Require Import distribution.
 Import uPred.
 
+Notation con_prob_lang_mdp := (con_lang_mdp con_prob_lang).
+
 Section adequacy.
+  Context `{!conerisGS Σ}.
 End adequacy.
+
+Class conerisGpreS Σ := ConerisGpreS {
+  conerisGpreS_iris  :: invGpreS Σ;
+  conerisGpreS_heap  :: ghost_mapG Σ loc val;
+  conerisGpreS_tapes :: ghost_mapG Σ loc tape;
+  conerisGpreS_err   :: ecGpreS Σ;
+}.
+
+Definition conerisΣ : gFunctors :=
+  #[invΣ; ghost_mapΣ loc val;
+    ghost_mapΣ loc tape;
+    GFunctor (authR nonnegrealUR)].
+Global Instance subG_conerisGPreS {Σ} : subG conerisΣ Σ → conerisGpreS Σ.
+Proof. solve_inG. Qed.
+
+Theorem wp_pgl Σ `{conerisGpreS Σ} `{Countable sch_int_state} (ζ : sch_int_state) n
+  (e : expr) (σ : state) (ε : R) (sch: scheduler con_prob_lang_mdp sch_int_state) φ :
+  0 <= ε →
+  (∀ `{conerisGS Σ}, ⊢ ↯ ε -∗ WP e {{ v, ⌜φ v⌝ }}) →
+  pgl (sch_exec sch n (ζ, ([e], σ))) φ ε.
+Proof.
+Admitted.
+
+Lemma pgl_closed_lim `{Countable sch_int_state} (ζ : sch_int_state) (e : expr) (σ : state) (ε : R)
+  (sch: scheduler con_prob_lang_mdp sch_int_state) φ :
+  (∀ n, pgl (sch_exec sch n (ζ, ([e], σ))) φ ε) →
+  pgl (sch_lim_exec sch (ζ, ([e], σ))) φ ε .
+Proof. intros Hn. by apply sch_lim_exec_continuous_prob. Qed.
+
+Theorem wp_pgl_lim Σ `{conerisGpreS Σ} `{Countable sch_int_state} (ζ : sch_int_state)
+  (e : expr) (σ : state) (ε : R) (sch: scheduler con_prob_lang_mdp sch_int_state) φ :
+  0 <= ε →
+  (∀ `{conerisGS Σ}, ⊢ ↯ ε -∗ WP e {{ v, ⌜φ v⌝ }}) →
+  pgl (sch_lim_exec sch (ζ, ([e], σ))) φ ε.
+Proof.
+  intros.
+  apply pgl_closed_lim.
+  intros.
+  by eapply wp_pgl.
+Qed.
+
+(* TODO limit stronger adequacy*)
